Wavelet/Determinacy/Congr.lean
@@ -169,8 +169,8 @@ theorem congr_eq_mod_ghost_proc_indexed_unguarded
     subst h₁ h₂ h₃
     have ⟨inputVals', _, hpop', heq_inputs, heq_chans'⟩ := congr_eq_mod_pop_vals heq_chans hpop
     cases hguard with
-    -- Normal operators
-    | triv_yield =>
+    -- Normal operators (w/ ghost tokens)
+    | triv_yield_ghost =>
       cases inputVals' using Vector.back_induction with
       | push inputVals' inputValsBack' ih =>
         replace ⟨heq_inputs, heq_back⟩ := Vector.forall₂_push_toList_to_forall₂ heq_inputs
@@ -190,7 +190,7 @@ theorem congr_eq_mod_ghost_proc_indexed_unguarded
         exact ⟨
           _,
           .step
-            (.idx_guard (.triv_yield (tok₂ := tok₂)))
+            (.idx_guard (.triv_yield_ghost (tok₂ := tok₂)))
             (.step_op
               (by simp [← heq_aps.length_eq, hi])
               hget'
@@ -204,6 +204,33 @@ theorem congr_eq_mod_ghost_proc_indexed_unguarded
               · simp [EqModGhost]
               · simp [EqModGhost]
         ⟩
+    -- Normal operators (w/o ghost tokens)
+    | triv_yield =>
+      simp [Vector.toList_map] at heq_inputs
+      have ⟨inputVals', h⟩ := Vector.forall₂_exists_map heq_inputs
+        (f := Sum.inl)
+        (by
+          intros x y heq
+          cases y <;> simp [EqModGhost] at heq
+          simp)
+      subst h
+      simp [Vector.toList_map, EqModGhost, Vector.toList_inj] at heq_inputs
+      simp [← heq_inputs] at hpop'
+      exact ⟨
+        _,
+        .step
+          (.idx_guard .triv_yield)
+          (.step_op
+            (by simp [← heq_aps.length_eq, hi])
+            hget'
+            hpop'),
+        by
+          constructor
+          · exact ⟨heq_proc_inputs, heq_proc_outputs, heq_aps⟩
+          · simp
+            apply congr_eq_mod_push_vals heq_chans'
+            simp [EqModGhost]
+      ⟩
     -- Calling join
     | triv_join =>
       rename_i toks vals outputToks _ _
@@ -437,20 +464,33 @@ theorem congr_eq_spec_guard
   cases l₁ with
   | yield op inputs outputs =>
     cases op with
-    | op op =>
+    | op ghost op =>
       cases hguard₁
-      rename_i inputs₁ outputs₁
-      generalize hinputs₁' :
-        (Vector.map Sum.inl inputs₁).push (Sum.inr (opSpec.pre op inputs₁)) = inputs₁'
-      generalize houtputs₁' :
-        (Vector.map Sum.inl outputs₁).push (Sum.inr (opSpec.post op inputs₁ outputs₁)) = outputs₁'
-      rw [hinputs₁', houtputs₁'] at hguard₂
-      cases hguard₂
-      rename_i inputs₂ outputs₂
-      simp [Vector.push_eq_push] at hinputs₁' houtputs₁'
-      have heq₁ := Vector.inj_map (by simp [Function.Injective]) hinputs₁'.2
-      have heq₂ := Vector.inj_map (by simp [Function.Injective]) houtputs₁'.2
-      simp [heq₁, heq₂]
+      case spec_yield_ghost =>
+        rename_i inputs₁ outputs₁
+        generalize hinputs₁' :
+          (Vector.map Sum.inl inputs₁).push (Sum.inr (opSpec.pre op inputs₁)) = inputs₁'
+        generalize houtputs₁' :
+          (Vector.map Sum.inl outputs₁).push (Sum.inr (opSpec.post op inputs₁ outputs₁)) = outputs₁'
+        rw [hinputs₁', houtputs₁'] at hguard₂
+        cases hguard₂
+        rename_i inputs₂ outputs₂
+        simp [Vector.push_eq_push] at hinputs₁' houtputs₁'
+        have heq₁ := Vector.inj_map (by simp [Function.Injective]) hinputs₁'.2
+        have heq₂ := Vector.inj_map (by simp [Function.Injective]) houtputs₁'.2
+        simp [heq₁, heq₂]
+      case spec_yield =>
+        rename_i inputs₁ outputs₁ _ _
+        generalize hinputs₁' :
+          Vector.map Sum.inl inputs₁ = inputs₁'
+        generalize houtputs₁' :
+          Vector.map Sum.inl outputs₁ = outputs₁'
+        rw [hinputs₁', houtputs₁'] at hguard₂
+        cases hguard₂
+        rename_i inputs₂ outputs₂
+        have heq₁ := Vector.inj_map (by simp [Function.Injective]) hinputs₁'
+        have heq₂ := Vector.inj_map (by simp [Function.Injective]) houtputs₁'
+        simp [heq₁, heq₂]
     | join k l req =>
       cases hguard₁ with | spec_join h₁ h₂ =>
       rename_i rem₁ toks₁ vals₁
@@ -499,11 +539,17 @@ theorem congr_eq_mod_ghost_triv_guard
     <;> cases hguard₂
     <;> simp [Label.EqMod] at heq
   any_goals rfl
-  case yield.yield.triv_yield.triv_yield =>
+  case yield.yield.triv_yield_ghost.triv_yield_ghost =>
     have ⟨h₁, heq₂, heq₃⟩ := heq
     subst h₁
     replace ⟨heq₂, _⟩ := Vector.forall₂_push_toList_to_forall₂ heq₂
     replace ⟨heq₃, _⟩ := Vector.forall₂_push_toList_to_forall₂ heq₃
+    simp [Vector.toList_map, EqModGhost, Vector.toList_inj] at heq₂
+    simp [Vector.toList_map, EqModGhost, Vector.toList_inj] at heq₃
+    simp [heq₂, heq₃]
+  case yield.yield.triv_yield.triv_yield =>
+    have ⟨h₁, heq₂, heq₃⟩ := heq
+    subst h₁
     simp [Vector.toList_map, EqModGhost, Vector.toList_inj] at heq₂
     simp [Vector.toList_map, EqModGhost, Vector.toList_inj] at heq₃
     simp [heq₂, heq₃]
